abp/ReceiverAutomaton.thy
@@ -3,13 +3,35 @@
  * This file was generated from Receiver.maa and will be overridden when changed. To change
  * permanently, consider changing the model itself.
  *
- * Generated on Oct 3, 2018 1:00:25 AM by isartransformer 1.0.0
+ * Generated on Oct 3, 2018 1:36:21 AM by isartransformer 1.0.0
  *)
 theory ReceiverAutomaton
   imports bundle.tsynBundle automat.dAutomaton
 
 begin
 
+
+(* TODO Move to tsynStream and find a name for it, the proposed "tsynmap_id" already exists *)
+lemma tsynmap_id_xx[simp]: "tsynDom\<cdot>tsyn \<subseteq> range F \<Longrightarrow> tsynMap F\<cdot>(tsynMap (inv F)\<cdot>tsyn) = tsyn"
+  apply(induction tsyn rule: ind)
+    apply simp_all
+  apply(rename_tac x xs)
+  apply(case_tac x)
+   apply(auto simp add: tsynmap_sconc_msg tsynmap_sconc_null)
+  by(auto simp add: tsyndom_sconc_msg tsyndom_sconc_null f_inv_into_f)
+
+(* TODO: Move to tsynBundle *)
+lemma tsynbundle_ctype: fixes ub::"'m::message tsyn SB"
+  shows "c\<in>ubDom\<cdot>ub \<Longrightarrow> tsynDom\<cdot>(ub . c) \<subseteq> (ctype c)"
+  apply(simp add: tsyndom_insert)
+  using usclOkay_stream_def ctype_tsyn_def
+  by (smt ctype_tsyn_iff mem_Collect_eq subsetCE subsetI ubdom_channel_usokay ubgetch_insert)
+
+(* TODO: Move to UBundle *)
+lemma ub_id_single: "ubDom\<cdot>ub = {c} \<Longrightarrow> Abs_ubundle [c \<mapsto> ub  .  c] = ub"
+  apply(rule ub_eq)
+  apply simp
+  by (simp add: ubWell_single_channel ubdom_ubrep_eq ubgetch_insert)+
 
 (* Helper for easier generation *)
 fun prepend :: "'a::type list \<Rightarrow> 'a \<Rightarrow> 'a list" where
@@ -20,7 +42,7 @@ section \<open>Datatype\<close>
 
 subsection \<open>Definition\<close>
 
-datatype ('e::countable) receiverMessage = DoNotUse_f2575d_ReceiverPair_E_Bool "('e\<times>bool)" | DoNotUse_f2575d_ReceiverBool "bool" | DoNotUse_f2575d_ReceiverE "'e"
+datatype ('e::countable) receiverMessage = DoNotUse_277815_ReceiverPair_E_Bool "('e\<times>bool)" | DoNotUse_277815_ReceiverBool "bool" | DoNotUse_277815_ReceiverE "'e"
 
 instance receiverMessage :: (countable) countable
   apply(intro_classes)
@@ -30,9 +52,9 @@ instantiation receiverMessage :: (countable) message
 begin
   fun ctype_receiverMessage :: "channel \<Rightarrow> ('e::countable) receiverMessage set" where
   "ctype_receiverMessage c = (
-    if c = \<C> ''DoNotUse_f2575d_dr'' then range DoNotUse_f2575d_ReceiverPair_E_Bool else
-    if c = \<C> ''DoNotUse_f2575d_ar'' then range DoNotUse_f2575d_ReceiverBool else
-    if c = \<C> ''DoNotUse_f2575d_o'' then range DoNotUse_f2575d_ReceiverE else
+    if c = \<C> ''DoNotUse_277815_dr'' then range DoNotUse_277815_ReceiverPair_E_Bool else
+    if c = \<C> ''DoNotUse_277815_ar'' then range DoNotUse_277815_ReceiverBool else
+    if c = \<C> ''DoNotUse_277815_o'' then range DoNotUse_277815_ReceiverE else
     undefined)"
   instance
     by(intro_classes)
@@ -42,10 +64,10 @@ end
 subsection \<open>Domain and Range\<close>
 
 definition receiverDom :: "channel set" where
-"receiverDom = {\<C> ''DoNotUse_f2575d_dr''}"
+"receiverDom = {\<C> ''DoNotUse_277815_dr''}"
 
 definition receiverRan :: "channel set" where
-"receiverRan = {\<C> ''DoNotUse_f2575d_ar'', \<C> ''DoNotUse_f2575d_o''}"
+"receiverRan = {\<C> ''DoNotUse_277815_ar'', \<C> ''DoNotUse_277815_o''}"
 
 
 section \<open>Setter\<close>
@@ -54,19 +76,19 @@ subsection \<open>type to sbElem\<close>
 
 (* Do not use this, use receiverElemIn_dr instead *)
 lift_definition receiverElem_raw_dr :: "('e\<times>bool) \<Rightarrow> ('e::countable) receiverMessage tsyn sbElem" is
-"\<lambda>x. [\<C> ''DoNotUse_f2575d_dr'' \<mapsto> Msg (DoNotUse_f2575d_ReceiverPair_E_Bool x)]"
+"\<lambda>x. [\<C> ''DoNotUse_277815_dr'' \<mapsto> Msg (DoNotUse_277815_ReceiverPair_E_Bool x)]"
   unfolding sbElemWell_def usclOkay_stream_def ctype_tsyn_def
   by simp
 
 (* Do not use this, use receiverElemOut_ar_o instead *)
 lift_definition receiverElem_raw_ar :: "bool \<Rightarrow> ('e::countable) receiverMessage tsyn sbElem" is
-"\<lambda>x. [\<C> ''DoNotUse_f2575d_ar'' \<mapsto> Msg (DoNotUse_f2575d_ReceiverBool x)]"
+"\<lambda>x. [\<C> ''DoNotUse_277815_ar'' \<mapsto> Msg (DoNotUse_277815_ReceiverBool x)]"
   unfolding sbElemWell_def usclOkay_stream_def ctype_tsyn_def
   by simp
 
 (* Do not use this, use receiverElemOut_ar_o instead *)
 lift_definition receiverElem_raw_o :: "'e \<Rightarrow> ('e::countable) receiverMessage tsyn sbElem" is
-"\<lambda>x. [\<C> ''DoNotUse_f2575d_o'' \<mapsto> Msg (DoNotUse_f2575d_ReceiverE x)]"
+"\<lambda>x. [\<C> ''DoNotUse_277815_o'' \<mapsto> Msg (DoNotUse_277815_ReceiverE x)]"
   unfolding sbElemWell_def usclOkay_stream_def ctype_tsyn_def
   by simp
 
@@ -78,17 +100,17 @@ subsubsection \<open>Intern\<close>
 (* Do not use this, use receiverElemIn_dr instead *)
 fun receiverElem_dr :: "('e\<times>bool) tsyn \<Rightarrow> ('e::countable) receiverMessage tsyn sbElem" where
 "receiverElem_dr (Msg port_dr) = receiverElem_raw_dr port_dr" |
-"receiverElem_dr null = sbeNull {\<C> ''DoNotUse_f2575d_dr''}"
+"receiverElem_dr null = sbeNull {\<C> ''DoNotUse_277815_dr''}"
 
 (* Do not use this, use receiverElemOut_ar_o instead *)
 fun receiverElem_ar :: "bool tsyn \<Rightarrow> ('e::countable) receiverMessage tsyn sbElem" where
 "receiverElem_ar (Msg port_ar) = receiverElem_raw_ar port_ar" |
-"receiverElem_ar null = sbeNull {\<C> ''DoNotUse_f2575d_ar''}"
+"receiverElem_ar null = sbeNull {\<C> ''DoNotUse_277815_ar''}"
 
 (* Do not use this, use receiverElemOut_ar_o instead *)
 fun receiverElem_o :: "'e tsyn \<Rightarrow> ('e::countable) receiverMessage tsyn sbElem" where
 "receiverElem_o (Msg port_o) = receiverElem_raw_o port_o" |
-"receiverElem_o null = sbeNull {\<C> ''DoNotUse_f2575d_o''}"
+"receiverElem_o null = sbeNull {\<C> ''DoNotUse_277815_o''}"
 
 declare receiverElem_dr.simps[simp del]
 
@@ -135,21 +157,21 @@ subsubsection \<open>Intern\<close>
 (* Do not use this, use receiverIn_list_dr instead *)
 fun receiver_list_dr :: "(('e\<times>bool) tsyn) list \<Rightarrow> ('e::countable) receiverMessage tsyn SB" where
 "receiver_list_dr (x#xs) = ubConcEq (receiver_dr x)\<cdot>(receiver_list_dr xs)" |
-"receiver_list_dr []     = ubLeast {\<C> ''DoNotUse_f2575d_dr''}"
+"receiver_list_dr []     = ubLeast {\<C> ''DoNotUse_277815_dr''}"
 
 declare receiver_list_dr.simps[simp del]
 
 (* Do not use this, use receiverOut_list_ar_o instead *)
 fun receiver_list_ar :: "(bool tsyn) list \<Rightarrow> ('e::countable) receiverMessage tsyn SB" where
 "receiver_list_ar (x#xs) = ubConcEq (receiver_ar x)\<cdot>(receiver_list_ar xs)" |
-"receiver_list_ar []     = ubLeast {\<C> ''DoNotUse_f2575d_ar''}"
+"receiver_list_ar []     = ubLeast {\<C> ''DoNotUse_277815_ar''}"
 
 declare receiver_list_ar.simps[simp del]
 
 (* Do not use this, use receiverOut_list_ar_o instead *)
 fun receiver_list_o :: "('e tsyn) list \<Rightarrow> ('e::countable) receiverMessage tsyn SB" where
 "receiver_list_o (x#xs) = ubConcEq (receiver_o x)\<cdot>(receiver_list_o xs)" |
-"receiver_list_o []     = ubLeast {\<C> ''DoNotUse_f2575d_o''}"
+"receiver_list_o []     = ubLeast {\<C> ''DoNotUse_277815_o''}"
 
 declare receiver_list_o.simps[simp del]
 
@@ -171,44 +193,44 @@ subsection \<open>stream to SB\<close>
 
 subsubsection \<open>Intern\<close>
 
-lift_definition DoNotUse_f2575d_receiver_stream_dr_h :: "('e\<times>bool) tsyn stream \<Rightarrow> ('e::countable) receiverMessage tsyn SB" is
-"\<lambda> s. [(\<C> ''DoNotUse_f2575d_dr'') \<mapsto> (tsynMap (DoNotUse_f2575d_ReceiverPair_E_Bool)\<cdot>s)]"
+lift_definition DoNotUse_277815_receiver_stream_dr_h :: "('e\<times>bool) tsyn stream \<Rightarrow> ('e::countable) receiverMessage tsyn SB" is
+"\<lambda> s. [(\<C> ''DoNotUse_277815_dr'') \<mapsto> (tsynMap (DoNotUse_277815_ReceiverPair_E_Bool)\<cdot>s)]"
   unfolding ubWell_def usclOkay_stream_def ctype_tsyn_def
   by auto
 
 (* Do not use this, use receiverIn_stream_dr instead *)
 lift_definition receiver_stream_dr :: "(('e\<times>bool)) tsyn stream \<rightarrow> ('e::countable) receiverMessage tsyn SB" is
-"DoNotUse_f2575d_receiver_stream_dr_h"
-  apply(auto simp add: cfun_def DoNotUse_f2575d_receiver_stream_dr_h_def map_fun_def comp_def)
+"DoNotUse_277815_receiver_stream_dr_h"
+  apply(auto simp add: cfun_def DoNotUse_277815_receiver_stream_dr_h_def map_fun_def comp_def)
   apply(rule cont_Abs_UB)
   apply(simp add: option_one_cont)
-  by (metis DoNotUse_f2575d_receiver_stream_dr_h.rep_eq ubrep_well)
+  by (metis DoNotUse_277815_receiver_stream_dr_h.rep_eq ubrep_well)
 
-lift_definition DoNotUse_f2575d_receiver_stream_ar_h :: "bool tsyn stream \<Rightarrow> ('e::countable) receiverMessage tsyn SB" is
-"\<lambda> s. [(\<C> ''DoNotUse_f2575d_ar'') \<mapsto> (tsynMap (DoNotUse_f2575d_ReceiverBool)\<cdot>s)]"
+lift_definition DoNotUse_277815_receiver_stream_ar_h :: "bool tsyn stream \<Rightarrow> ('e::countable) receiverMessage tsyn SB" is
+"\<lambda> s. [(\<C> ''DoNotUse_277815_ar'') \<mapsto> (tsynMap (DoNotUse_277815_ReceiverBool)\<cdot>s)]"
   unfolding ubWell_def usclOkay_stream_def ctype_tsyn_def
   by auto
 
 (* Do not use this, use receiverOut_stream_ar_o instead *)
 lift_definition receiver_stream_ar :: "(bool) tsyn stream \<rightarrow> ('e::countable) receiverMessage tsyn SB" is
-"DoNotUse_f2575d_receiver_stream_ar_h"
-  apply(auto simp add: cfun_def DoNotUse_f2575d_receiver_stream_ar_h_def map_fun_def comp_def)
+"DoNotUse_277815_receiver_stream_ar_h"
+  apply(auto simp add: cfun_def DoNotUse_277815_receiver_stream_ar_h_def map_fun_def comp_def)
   apply(rule cont_Abs_UB)
   apply(simp add: option_one_cont)
-  by (metis DoNotUse_f2575d_receiver_stream_ar_h.rep_eq ubrep_well)
+  by (metis DoNotUse_277815_receiver_stream_ar_h.rep_eq ubrep_well)
 
-lift_definition DoNotUse_f2575d_receiver_stream_o_h :: "'e tsyn stream \<Rightarrow> ('e::countable) receiverMessage tsyn SB" is
-"\<lambda> s. [(\<C> ''DoNotUse_f2575d_o'') \<mapsto> (tsynMap (DoNotUse_f2575d_ReceiverE)\<cdot>s)]"
+lift_definition DoNotUse_277815_receiver_stream_o_h :: "'e tsyn stream \<Rightarrow> ('e::countable) receiverMessage tsyn SB" is
+"\<lambda> s. [(\<C> ''DoNotUse_277815_o'') \<mapsto> (tsynMap (DoNotUse_277815_ReceiverE)\<cdot>s)]"
   unfolding ubWell_def usclOkay_stream_def ctype_tsyn_def
   by auto
 
 (* Do not use this, use receiverOut_stream_ar_o instead *)
 lift_definition receiver_stream_o :: "('e) tsyn stream \<rightarrow> ('e::countable) receiverMessage tsyn SB" is
-"DoNotUse_f2575d_receiver_stream_o_h"
-  apply(auto simp add: cfun_def DoNotUse_f2575d_receiver_stream_o_h_def map_fun_def comp_def)
+"DoNotUse_277815_receiver_stream_o_h"
+  apply(auto simp add: cfun_def DoNotUse_277815_receiver_stream_o_h_def map_fun_def comp_def)
   apply(rule cont_Abs_UB)
   apply(simp add: option_one_cont)
-  by (metis DoNotUse_f2575d_receiver_stream_o_h.rep_eq ubrep_well)
+  by (metis DoNotUse_277815_receiver_stream_o_h.rep_eq ubrep_well)
 
 
 subsubsection \<open>In/Out\<close>
@@ -226,27 +248,27 @@ section \<open>Getter\<close>
 subsection \<open>sbElem to tsyn\<close>
 
 definition receiverElem_get_dr :: "('e::countable) receiverMessage tsyn sbElem \<Rightarrow> (('e\<times>bool)) tsyn" where
-"receiverElem_get_dr sbe = tsynApplyElem (inv DoNotUse_f2575d_ReceiverPair_E_Bool) ((Rep_sbElem sbe) \<rightharpoonup> (\<C> ''DoNotUse_f2575d_dr''))"
+"receiverElem_get_dr sbe = tsynApplyElem (inv DoNotUse_277815_ReceiverPair_E_Bool) ((Rep_sbElem sbe) \<rightharpoonup> (\<C> ''DoNotUse_277815_dr''))"
 
 definition receiverElem_get_ar :: "('e::countable) receiverMessage tsyn sbElem \<Rightarrow> (bool) tsyn" where
-"receiverElem_get_ar sbe = tsynApplyElem (inv DoNotUse_f2575d_ReceiverBool) ((Rep_sbElem sbe) \<rightharpoonup> (\<C> ''DoNotUse_f2575d_ar''))"
+"receiverElem_get_ar sbe = tsynApplyElem (inv DoNotUse_277815_ReceiverBool) ((Rep_sbElem sbe) \<rightharpoonup> (\<C> ''DoNotUse_277815_ar''))"
 
 definition receiverElem_get_o :: "('e::countable) receiverMessage tsyn sbElem \<Rightarrow> ('e) tsyn" where
-"receiverElem_get_o sbe = tsynApplyElem (inv DoNotUse_f2575d_ReceiverE) ((Rep_sbElem sbe) \<rightharpoonup> (\<C> ''DoNotUse_f2575d_o''))"
+"receiverElem_get_o sbe = tsynApplyElem (inv DoNotUse_277815_ReceiverE) ((Rep_sbElem sbe) \<rightharpoonup> (\<C> ''DoNotUse_277815_o''))"
 
 
 subsection \<open>SB to stream\<close>
 
 lift_definition receiver_get_stream_dr :: "('e::countable) receiverMessage tsyn SB \<rightarrow> ('e\<times>bool) tsyn stream" is
-"\<lambda>sb. tsynMap (inv DoNotUse_f2575d_ReceiverPair_E_Bool)\<cdot>(sb . (\<C> ''DoNotUse_f2575d_dr''))"
+"\<lambda>sb. tsynMap (inv DoNotUse_277815_ReceiverPair_E_Bool)\<cdot>(sb . (\<C> ''DoNotUse_277815_dr''))"
   by(simp add: cfun_def)
 
 lift_definition receiver_get_stream_ar :: "('e::countable) receiverMessage tsyn SB \<rightarrow> bool tsyn stream" is
-"\<lambda>sb. tsynMap (inv DoNotUse_f2575d_ReceiverBool)\<cdot>(sb . (\<C> ''DoNotUse_f2575d_ar''))"
+"\<lambda>sb. tsynMap (inv DoNotUse_277815_ReceiverBool)\<cdot>(sb . (\<C> ''DoNotUse_277815_ar''))"
   by(simp add: cfun_def)
 
 lift_definition receiver_get_stream_o :: "('e::countable) receiverMessage tsyn SB \<rightarrow> 'e tsyn stream" is
-"\<lambda>sb. tsynMap (inv DoNotUse_f2575d_ReceiverE)\<cdot>(sb . (\<C> ''DoNotUse_f2575d_o''))"
+"\<lambda>sb. tsynMap (inv DoNotUse_277815_ReceiverE)\<cdot>(sb . (\<C> ''DoNotUse_277815_o''))"
   by(simp add: cfun_def)
 
 
@@ -335,34 +357,34 @@ subsection \<open>tsyn to sbElem/SB\<close>
 
 subsubsection \<open>Intern\<close>
 
-lemma receiverelem_dr_dom[simp]: "sbeDom (receiverElem_dr x) = {\<C> ''DoNotUse_f2575d_dr''}"
+lemma receiverelem_dr_dom[simp]: "sbeDom (receiverElem_dr x) = {\<C> ''DoNotUse_277815_dr''}"
   apply(cases x)
   apply(simp add: receiverElem_dr.simps sbeDom_def receiverElem_raw_dr.rep_eq)
   by(simp add: receiverElem_dr.simps)
 
-lemma receiverelem_ar_dom[simp]: "sbeDom (receiverElem_ar x) = {\<C> ''DoNotUse_f2575d_ar''}"
+lemma receiverelem_ar_dom[simp]: "sbeDom (receiverElem_ar x) = {\<C> ''DoNotUse_277815_ar''}"
   apply(cases x)
   apply(simp add: receiverElem_ar.simps sbeDom_def receiverElem_raw_ar.rep_eq)
   by(simp add: receiverElem_ar.simps)
 
-lemma receiverelem_o_dom[simp]: "sbeDom (receiverElem_o x) = {\<C> ''DoNotUse_f2575d_o''}"
+lemma receiverelem_o_dom[simp]: "sbeDom (receiverElem_o x) = {\<C> ''DoNotUse_277815_o''}"
   apply(cases x)
   apply(simp add: receiverElem_o.simps sbeDom_def receiverElem_raw_o.rep_eq)
   by(simp add: receiverElem_o.simps)
 
-lemma receiver_dr_dom[simp]: "ubDom\<cdot>(receiver_dr x) = {\<C> ''DoNotUse_f2575d_dr''}"
+lemma receiver_dr_dom[simp]: "ubDom\<cdot>(receiver_dr x) = {\<C> ''DoNotUse_277815_dr''}"
   by(simp add: receiver_dr_def)
 
 lemma receiver_dr_len[simp]: "ubLen (receiver_dr x) = 1"
   by(simp add: receiver_dr_def)
 
-lemma receiver_ar_dom[simp]: "ubDom\<cdot>(receiver_ar x) = {\<C> ''DoNotUse_f2575d_ar''}"
+lemma receiver_ar_dom[simp]: "ubDom\<cdot>(receiver_ar x) = {\<C> ''DoNotUse_277815_ar''}"
   by(simp add: receiver_ar_def)
 
 lemma receiver_ar_len[simp]: "ubLen (receiver_ar x) = 1"
   by(simp add: receiver_ar_def)
 
-lemma receiver_o_dom[simp]: "ubDom\<cdot>(receiver_o x) = {\<C> ''DoNotUse_f2575d_o''}"
+lemma receiver_o_dom[simp]: "ubDom\<cdot>(receiver_o x) = {\<C> ''DoNotUse_277815_o''}"
   by(simp add: receiver_o_def)
 
 lemma receiver_o_len[simp]: "ubLen (receiver_o x) = 1"
@@ -394,35 +416,62 @@ subsection \<open>stream to SB\<close>
 
 subsubsection \<open>Intern\<close>
 
-lemma receiver_stream_dr_dom[simp]: "ubDom\<cdot>(receiver_stream_dr\<cdot>x) = {\<C> ''DoNotUse_f2575d_dr''}"
-  by(simp add: receiver_stream_dr.rep_eq ubdom_insert DoNotUse_f2575d_receiver_stream_dr_h.rep_eq)
+lemma receiver_stream_dr_dom[simp]: "ubDom\<cdot>(receiver_stream_dr\<cdot>x) = {\<C> ''DoNotUse_277815_dr''}"
+  by(simp add: receiver_stream_dr.rep_eq ubdom_insert DoNotUse_277815_receiver_stream_dr_h.rep_eq)
 
 lemma receiver_stream_dr_len[simp]: "ubLen (receiver_stream_dr\<cdot>x) = #x"
   apply(subst uslen_ubLen_ch3)
   apply simp
   apply(simp add: receiver_stream_dr.rep_eq)
-  apply(simp add: ubGetCh_def DoNotUse_f2575d_receiver_stream_dr_h.rep_eq)
+  apply(simp add: ubGetCh_def DoNotUse_277815_receiver_stream_dr_h.rep_eq)
   by (simp add: tsynmap_slen usclLen_stream_def)
 
-lemma receiver_stream_ar_dom[simp]: "ubDom\<cdot>(receiver_stream_ar\<cdot>x) = {\<C> ''DoNotUse_f2575d_ar''}"
-  by(simp add: receiver_stream_ar.rep_eq ubdom_insert DoNotUse_f2575d_receiver_stream_ar_h.rep_eq)
+lemma receiver_stream_dr_id[simp]:
+  assumes "ubDom\<cdot>ub = {\<C> ''DoNotUse_277815_dr''} "
+    shows "receiver_stream_dr\<cdot>(receiver_get_stream_dr\<cdot>ub) = ub"
+  apply(simp add: receiver_stream_dr.rep_eq receiver_get_stream_dr.rep_eq)
+  apply(simp add: DoNotUse_277815_receiver_stream_dr_h_def)
+  apply(subst tsynmap_id_xx)
+  using assms tsynbundle_ctype apply fastforce
+  using assms ub_id_single by blast
+
+lemma receiver_stream_ar_dom[simp]: "ubDom\<cdot>(receiver_stream_ar\<cdot>x) = {\<C> ''DoNotUse_277815_ar''}"
+  by(simp add: receiver_stream_ar.rep_eq ubdom_insert DoNotUse_277815_receiver_stream_ar_h.rep_eq)
 
 lemma receiver_stream_ar_len[simp]: "ubLen (receiver_stream_ar\<cdot>x) = #x"
   apply(subst uslen_ubLen_ch3)
   apply simp
   apply(simp add: receiver_stream_ar.rep_eq)
-  apply(simp add: ubGetCh_def DoNotUse_f2575d_receiver_stream_ar_h.rep_eq)
+  apply(simp add: ubGetCh_def DoNotUse_277815_receiver_stream_ar_h.rep_eq)
   by (simp add: tsynmap_slen usclLen_stream_def)
 
-lemma receiver_stream_o_dom[simp]: "ubDom\<cdot>(receiver_stream_o\<cdot>x) = {\<C> ''DoNotUse_f2575d_o''}"
-  by(simp add: receiver_stream_o.rep_eq ubdom_insert DoNotUse_f2575d_receiver_stream_o_h.rep_eq)
+lemma receiver_stream_ar_id[simp]:
+  assumes "ubDom\<cdot>ub = {\<C> ''DoNotUse_277815_ar''} "
+    shows "receiver_stream_ar\<cdot>(receiver_get_stream_ar\<cdot>ub) = ub"
+  apply(simp add: receiver_stream_ar.rep_eq receiver_get_stream_ar.rep_eq)
+  apply(simp add: DoNotUse_277815_receiver_stream_ar_h_def)
+  apply(subst tsynmap_id_xx)
+  using assms tsynbundle_ctype apply fastforce
+  using assms ub_id_single by blast
+
+lemma receiver_stream_o_dom[simp]: "ubDom\<cdot>(receiver_stream_o\<cdot>x) = {\<C> ''DoNotUse_277815_o''}"
+  by(simp add: receiver_stream_o.rep_eq ubdom_insert DoNotUse_277815_receiver_stream_o_h.rep_eq)
 
 lemma receiver_stream_o_len[simp]: "ubLen (receiver_stream_o\<cdot>x) = #x"
   apply(subst uslen_ubLen_ch3)
   apply simp
   apply(simp add: receiver_stream_o.rep_eq)
-  apply(simp add: ubGetCh_def DoNotUse_f2575d_receiver_stream_o_h.rep_eq)
+  apply(simp add: ubGetCh_def DoNotUse_277815_receiver_stream_o_h.rep_eq)
   by (simp add: tsynmap_slen usclLen_stream_def)
+
+lemma receiver_stream_o_id[simp]:
+  assumes "ubDom\<cdot>ub = {\<C> ''DoNotUse_277815_o''} "
+    shows "receiver_stream_o\<cdot>(receiver_get_stream_o\<cdot>ub) = ub"
+  apply(simp add: receiver_stream_o.rep_eq receiver_get_stream_o.rep_eq)
+  apply(simp add: DoNotUse_277815_receiver_stream_o_h_def)
+  apply(subst tsynmap_id_xx)
+  using assms tsynbundle_ctype apply fastforce
+  using assms ub_id_single by blast
 
 
 subsubsection \<open>In/Out\<close>
@@ -488,17 +537,17 @@ subsubsection \<open>Intern\<close>
 
 lemma receiver_stream_dr_id[simp]: "receiver_get_stream_dr\<cdot>(receiver_stream_dr\<cdot>x) = x"
   apply(simp add: receiver_get_stream_dr.rep_eq receiver_stream_dr.rep_eq)
-  apply(simp add: ubGetCh_def DoNotUse_f2575d_receiver_stream_dr_h.rep_eq)
+  apply(simp add: ubGetCh_def DoNotUse_277815_receiver_stream_dr_h.rep_eq)
   by (simp add: inj_def)
 
 lemma receiver_stream_ar_id[simp]: "receiver_get_stream_ar\<cdot>(receiver_stream_ar\<cdot>x) = x"
   apply(simp add: receiver_get_stream_ar.rep_eq receiver_stream_ar.rep_eq)
-  apply(simp add: ubGetCh_def DoNotUse_f2575d_receiver_stream_ar_h.rep_eq)
+  apply(simp add: ubGetCh_def DoNotUse_277815_receiver_stream_ar_h.rep_eq)
   by (simp add: inj_def)
 
 lemma receiver_stream_o_id[simp]: "receiver_get_stream_o\<cdot>(receiver_stream_o\<cdot>x) = x"
   apply(simp add: receiver_get_stream_o.rep_eq receiver_stream_o.rep_eq)
-  apply(simp add: ubGetCh_def DoNotUse_f2575d_receiver_stream_o_h.rep_eq)
+  apply(simp add: ubGetCh_def DoNotUse_277815_receiver_stream_o_h.rep_eq)
   by (simp add: inj_def)
 
 
